SP1Foundations/Constraint.lean
@@ -28,51 +28,55 @@ inductive SP1Constraint where
   | send (interaction : AirInteraction) (mult : BabyBear)
   /-- Receiving an air interaction -/
   | receive (interaction : AirInteraction) (mult : BabyBear)
-  deriving DecidableEq
+  | funcall (res : List SP1Constraint)
+  /- deriving DecidableEq -/
 
 namespace SP1Constraint
 
 def toProp : SP1Constraint → Prop
   | .assertZero x => (x = 0)
   | .send (.byte op a b c) (mult) => mult = 1 → op.constrain a b c
-  | _ => false
+  | .receive (.memory _ _ _ low_limb high_limb) (mult) =>
+      mult = 1 → (low_limb < 65536 ∧ high_limb < 65536)
+  | .funcall lst => List.Forall toProp lst
+  | _ => 1 = 1
 
-@[simp] lemma toProp_assertZero (x : BabyBear) :
-    (assertZero x).toProp ↔ x = 0 := Iff.rfl
-
-@[simp] lemma toProp_sendAirInteration_byte (op : ByteOpcode)
-    (a b c mult : BabyBear) :
-    (send (.byte op a b c) mult).toProp ↔
-      (mult = 1 → ByteOpcode.constrain op a b c) := Iff.rfl
+/- @[simp] lemma toProp_assertZero (x : BabyBear) : -/
+/-     (assertZero x).toProp ↔ x = 0 := Iff.rfl -/
+/--/
+/- @[simp] lemma toProp_sendAirInteration_byte (op : ByteOpcode) -/
+/-     (a b c mult : BabyBear) : -/
+/-     (send (.byte op a b c) mult).toProp ↔ -/
+/-       (mult = 1 → ByteOpcode.constrain op a b c) := Iff.rfl -/
 
 end SP1Constraint
 
-section constraintSet
-
--- TODO: should this exist? maybe even as `abbrev`?
-@[reducible] def constraintSet := Finset SP1Constraint
-
-/-- Covert a set of constraints to a single proposition stating that they all hold. -/
-def constraintSet_toProp (cs : Finset SP1Constraint) : Prop :=
-  ∀ constraint ∈ cs, constraint.toProp
-
-@[simp] lemma constraintSet_toProp_empty : constraintSet_toProp ∅ = True := by
-  simp [constraintSet_toProp]
-
-@[simp] lemma constraintSet_toProp_singleton (c : SP1Constraint) : constraintSet_toProp {c} = c.toProp := by
-  simp [constraintSet_toProp]
-
-@[simp] lemma constraintSet_toProp_insert (c : SP1Constraint) (cs : Finset SP1Constraint) :
-    constraintSet_toProp (insert c cs) = (c.toProp ∧ constraintSet_toProp cs) := by
-  simp [constraintSet_toProp]
-
-lemma toProp_of_mem_constraintSet (cs : Finset SP1Constraint) (c : SP1Constraint) :
-    c ∈ cs → constraintSet_toProp cs → c.toProp := by
-  aesop
-
-/-- A larger set of constraints `cs'` implies a smaller set of constraints `cs`. -/
-lemma toProp_imp_of_constraintSet_subset' (cs cs' : Finset SP1Constraint)
-    (h : cs ⊆ cs') : constraintSet_toProp cs' → constraintSet_toProp cs := by
-  refine fun csp c h' => csp c (h h')
-
-end constraintSet
+-- section constraintSet
+-- 
+-- -- TODO: should this exist? maybe even as `abbrev`?
+-- @[reducible] def constraintSet := Finset SP1Constraint
+-- 
+-- /-- Covert a set of constraints to a single proposition stating that they all hold. -/
+-- def constraintSet_toProp (cs : Finset SP1Constraint) : Prop :=
+--   ∀ constraint ∈ cs, constraint.toProp
+-- 
+-- @[simp] lemma constraintSet_toProp_empty : constraintSet_toProp ∅ = True := by
+--   simp [constraintSet_toProp]
+-- 
+-- @[simp] lemma constraintSet_toProp_singleton (c : SP1Constraint) : constraintSet_toProp {c} = c.toProp := by
+--   simp [constraintSet_toProp]
+-- 
+-- @[simp] lemma constraintSet_toProp_insert (c : SP1Constraint) (cs : Finset SP1Constraint) :
+--     constraintSet_toProp (insert c cs) = (c.toProp ∧ constraintSet_toProp cs) := by
+--   simp [constraintSet_toProp]
+-- 
+-- lemma toProp_of_mem_constraintSet (cs : Finset SP1Constraint) (c : SP1Constraint) :
+--     c ∈ cs → constraintSet_toProp cs → c.toProp := by
+--   aesop
+-- 
+-- /-- A larger set of constraints `cs'` implies a smaller set of constraints `cs`. -/
+-- lemma toProp_imp_of_constraintSet_subset' (cs cs' : Finset SP1Constraint)
+--     (h : cs ⊆ cs') : constraintSet_toProp cs' → constraintSet_toProp cs := by
+--   refine fun csp c h' => csp c (h h')
+-- 
+-- end constraintSet
