SP1Operations/CPUState.lean
@@ -15,10 +15,23 @@ namespace CPUState
 
 def clk (cols : CPUState) : BabyBear := 2^14 * cols.clk_high_limb + cols.clk_low_limb
 
-def spec
+def constraints
   (cols : CPUState)
   (next_pc : BabyBear)
   (clk_increment : BabyBear)
-  (is_real : U1) : Prop := by sorry
+  (is_real : BabyBear)
+  : List SP1Constraint :=
+  let E0 : BabyBear := 16384 * cols.clk_high_limb
+  let E2 : BabyBear := E0 + cols.clk_low_limb
+  let E4 : BabyBear := is_real - 1
+  let E6 : BabyBear := is_real * E4
+  let E8 : BabyBear := E2 + clk_increment
+  [
+    .assertZero E6,
+    .receive (.state cols.shard E2 cols.pc) is_real,
+    .send (.state cols.shard E8 next_pc) is_real,
+    .send (.byte ByteOpcode.Range cols.clk_high_limb 14 0) is_real,
+    .send (.byte ByteOpcode.Range cols.clk_low_limb 14 0) is_real
+  ]
 
 end CPUState
