SP1Operations/RTypeReader.lean
@@ -5,43 +5,75 @@ import LeanRV32D.RiscvRegs
 open LeanRV32D.Functions
 
 --- A Reader that only accesses values of type `T`.
-structure RTypeReader (T : Type) where
-  op_a : T 
-  op_a_memory : MemoryAccessInSharedCols T
-  op_a_0 : T
-  op_b : T 
-  op_b_memory : MemoryAccessInSharedCols T
-  op_c : T 
-  op_c_memory : MemoryAccessInSharedCols T
+structure RTypeReader where
+  op_a : BabyBear
+  op_a_memory : MemoryAccessInSharedCols
+  op_a_0 : BabyBear
+  op_b : BabyBear
+  op_b_memory : MemoryAccessInSharedCols
+  op_c : BabyBear
+  op_c_memory : MemoryAccessInSharedCols
 
 namespace RTypeReader 
 
-def b {T : Type} (cols : RTypeReader T) : Word T := cols.op_b_memory.prev_value
+/- def b {T : Type} (cols : RTypeReader T) : Word T := cols.op_b_memory.prev_value -/
+/- def c {T : Type} (cols : RTypeReader T) : Word T := cols.op_c_memory.prev_value -/
 
-def c {T : Type} (cols : RTypeReader T) : Word T := cols.op_c_memory.prev_value
+def constraints
+  (shard clk pc opcode: BabyBear)
+  (op_a_write_value : Word BabyBear)
+  (cols : RTypeReader)
+  (is_real : BabyBear)
+  : List SP1Constraint :=
+  let E0 : BabyBear := is_real - 1
+  let E2 : BabyBear := is_real * E0
+  let E4 : BabyBear := 0 + cols.op_b
+  let E6 : BabyBear := 0 + cols.op_c
+  let E8 : BabyBear := op_a_write_value[0] - 0
+  let E10 : BabyBear := cols.op_a_0 * E8
+  let E12 : BabyBear := op_a_write_value[1] - 0
+  let E14 : BabyBear := cols.op_a_0 * E12
+  let E16 : BabyBear := clk + 3
+  let E18 : BabyBear := is_real - 1
+  let E20 : BabyBear := is_real * E18
+  let E22 : BabyBear := E16 - cols.op_a_memory.access_timestamp.prev_clk
+  let E24 : BabyBear := E22 - 1
+  let E26 : BabyBear := E24 - cols.op_a_memory.access_timestamp.diff_low_limb
+  let E28 : BabyBear := E26 * 2013143041
+  let E30 : BabyBear := clk + 2
+  let E32 : BabyBear := is_real - 1
+  let E34 : BabyBear := is_real * E32
+  let E36 : BabyBear := E30 - cols.op_b_memory.access_timestamp.prev_clk
+  let E38 : BabyBear := E36 - 1
+  let E40 : BabyBear := E38 - cols.op_b_memory.access_timestamp.diff_low_limb
+  let E42 : BabyBear := E40 * 2013143041
+  let E44 : BabyBear := clk + 1
+  let E46 : BabyBear := is_real - 1
+  let E48 : BabyBear := is_real * E46
+  let E50 : BabyBear := E44 - cols.op_c_memory.access_timestamp.prev_clk
+  let E52 : BabyBear := E50 - 1
+  let E54 : BabyBear := E52 - cols.op_c_memory.access_timestamp.diff_low_limb
+  let E56 : BabyBear := E54 * 2013143041
 
-def spec {T : Type}
-  (cols : RTypeReader T)
-  (shard : BabyBear)
-  (clk : BabyBear)
-  (pc : BabyBear)
-  (opcode : BabyBear)
-  (op_a_write_value : Word T)
-  (is_real : U1)
-  : Prop := sorry
-
-def read_b_fun
-  (cols : RTypeReader U16)
-  (rs : regidx)
-  : Prop := rX_bits rs = pure cols.b.toBV32_U16
-
-def read_c_fun
-  (cols : RTypeReader U16)
-  (rs : regidx)
-  : Prop := rX_bits rs = pure cols.c.toBV32_U16
+  [
+    .assertZero E2,
+    .assertZero E10,
+    .assertZero E14,
+    .assertZero E20,
+    .send (.byte ByteOpcode.Range cols.op_a_memory.access_timestamp.diff_low_limb 14 0) is_real,
+    .send (.byte ByteOpcode.Range E28 14 0) is_real,
+    .send (.memory shard cols.op_a_memory.access_timestamp.prev_clk cols.op_a cols.op_a_memory.prev_value[0] cols.op_a_memory.prev_value[1]) is_real,
+    .receive (.memory shard E16 cols.op_a op_a_write_value[0] op_a_write_value[1]) is_real,
+    .assertZero E34,
+    .send (.byte ByteOpcode.Range cols.op_b_memory.access_timestamp.diff_low_limb 14 0) is_real,
+    .send (.byte ByteOpcode.Range E42 14 0) is_real,
+    .send (.memory shard cols.op_b_memory.access_timestamp.prev_clk cols.op_b cols.op_b_memory.prev_value[0] cols.op_b_memory.prev_value[1]) is_real,
+    .receive (.memory shard E30 cols.op_b cols.op_b_memory.prev_value[0] cols.op_b_memory.prev_value[1]) is_real,
+    .assertZero E48,
+    .send (.byte ByteOpcode.Range cols.op_c_memory.access_timestamp.diff_low_limb 14 0) is_real,
+    .send (.byte ByteOpcode.Range E56 14 0) is_real,
+    .send (.memory shard cols.op_c_memory.access_timestamp.prev_clk cols.op_c cols.op_c_memory.prev_value[0] cols.op_c_memory.prev_value[1]) is_real,
+    .receive (.memory shard E44 cols.op_c cols.op_c_memory.prev_value[0] cols.op_c_memory.prev_value[1]) is_real
+  ]
 
 end RTypeReader
-
-structure MemRead (x : Word U16) where
-  val : BitVec 32
-  h_val : val = x.toBV32_U16
