SP1Operations/MemoryConsistency.lean
@@ -7,6 +7,6 @@ structure MemoryAccessInShardTimestamp where
 -- MemoryAccessInSharedCols is parameterized on type `T` because we may want to
 -- dynamically enforce that `prev_value` is specifically some width, e.g. U16 or
 -- U8, etc.
-structure MemoryAccessInSharedCols (T : Type) where
-  prev_value : Word T
+structure MemoryAccessInSharedCols where
+  prev_value : Word BabyBear
   access_timestamp : MemoryAccessInShardTimestamp
